new language

Transformation.v
@@ -7,7 +7,7 @@ Basic transformations.
 
 Set Implicit Arguments.
 
-Require Export LambdaSemantics.
+Require Export Semantics.
 
 (*
 Definition is_add_zero t : option trm :=
@@ -17,61 +17,83 @@ Definition is_add_zero t : option trm :=
   end.
 
 Lemma is_add_zero_some : forall t1 t2 t m1 m2 v,
-  is_add_zero t1 t2 = Some t -> 
-  red m1 (trm_app t1 t2) m2 v -> 
+  is_add_zero t1 t2 = Some t ->
+  red m1 (trm_app t1 t2) m2 v ->
   red m1 t m2 v.
-Proof. 
-  introv M R. unfolds is_add_zero. 
+Proof.
+  introv M R. unfolds is_add_zero.
   destruct t1; tryfalse. destruct t1_1; tryfalse.
   destruct v0; tryfalse. destruct p; tryfalse.
   destruct t1_2; tryfalse. destruct v0; tryfalse.
   destruct z; tryfalse. inverts M. Search val_add.
-  inverts R. 
+  inverts R.
   { inverts H1. inverts H3. }
   { asserts_rewrite (0 + n2 = n2). math. constructor. }
 Qed.
 *)
 
+Global Instance Inhab_trm : Inhab trm.
+Proof using. apply (Inhab_of_val (trm_val val_unit)). Qed.
+
 
 (* Remove plus zero, i.e. t + 0 = t and 0 + t = t *)
-Fixpoint transf_rm_pz (t:trm) : trm :=
-  let aux := transf_rm_pz in
+Fixpoint tr (t:trm) : trm :=
+  let aux := tr in
   match t with
   | trm_val v => trm_val v
   | trm_var x => trm_var x
-  (* | trm_fix b1 b2 t1 => trm_fix b1 b2 (aux t1) *)
-  | trm_if t1 t2 t3 => 
+  | trm_if t1 t2 t3 =>
       trm_if (aux t1) (aux t2) (aux t3)
-  | trm_let b t1 t2 => 
+  | trm_let b t1 t2 =>
       trm_let b (aux t1) (aux t2)
-  | trm_app t1 t2 => trm_app (aux t1) (aux t2)
-     (*  let t1' := aux t1 in
-      let t2' := aux t2 in
-      match is_add_zero t1' t2' with
-      | Some t => t
-      | None => trm_app t1' t2'
-      end*)
-  | trm_binop op t1 t2 => 
-    match op, t1, t2 with
-    | binop_add, val_int 0, t2 => aux t2
-    (* | binop_add, t1, val_int 0 => aux t1 *)
-    | _, _, _  => trm_binop op (aux t1) (aux t2)
-    end
-  | trm_while t1 t2 => trm_while (aux t1) (aux t2)
-  | trm_for v t1 t2 t3 => 
-      trm_for v t(aux t1) (aux t2) (aux t3)
+  | trm_app f ts => 
+      let ts' := List.map aux ts in
+      if isTrue (f = binop_add /\ exists t2, ts' = (trm_val 0)::t2::nil)  (* k = t2::nil *)
+        then LibList.nth 1 ts'
+        else trm_app f ts'
   end.
-  
+
+
+Theorem red_tr: forall E t s1 s2 v,
+  red E s1 t s2 v -> 
+  red E s1 (tr t) s2 v.
+Proof.
+  introv R. induction R; simpl. (*  try solve [ try case_if; constructors* ]. *)
+  { constructors*. }
+  { constructors*. }
+  { eapply red_if.
+    { eauto. }
+    { case_if*. } }
+  { constructors*. }
+  { case_if.
+     { destruct C as (C1&(k&C2)). inverts C1. inverts H.
+        inverts C2. rew_listx. math_rewrite (0 + n2 = n2). constructor~. }
+     { rew_logic in *. constructors*. } } }
+  (* todo : optimize *)
+  { case_if as C; [rew_logic in C; destruct C; tryfalse | ]. constructors*.  }
+  { case_if as C; [rew_logic in C; destruct C; tryfalse | ]. constructors*.  }
+  { case_if as C; [rew_logic in C; destruct C; tryfalse | ]. constructors*.  }
+Qed.
+
+
+
+
+
+(* 
+  | trm_while t1 t2 => trm_while (aux t1) (aux t2)
+  | trm_for v t1 t2 t3 =>
+      trm_for v t(aux t1) (aux t2) (aux t3)
+*)
 
 Print transf_rm_pz.
 
-Example simple_example_1: 
+Example simple_example_1:
   transf_rm_pz (val_add (val_int 0) (val_int 5)) = val_int 5.
 Proof.
   simpl. reflexivity.
 Qed.
 
-(*Example simple_example_2: 
+(*Example simple_example_2:
   transf_rm_pz (val_add (val_int 5) (val_int 0)) = val_int 5.
 Proof.
   simpl. reflexivity.
@@ -97,13 +119,13 @@ Admitted.
 Lemma transf_subst_commute: forall b v t,
   subst1 b v (transf_rm_pz t) = transf_rm_pz (subst1 b v t).
 Proof.
-  intros. rewrite subst1_eq_subst1'. 
+  intros. rewrite subst1_eq_subst1'.
   induction t; simpl. (*try solve [fequal; try case_if; auto].*)
   { auto. }
   { case_if; simpl; auto. }
   { admit. }
-  { fequal*. } 
-  { fequal. 
+  { fequal*. }
+  { fequal.
     { eauto. }
     { case_if; eauto. }}
   { rewrite <- IHt1, <- IHt2. admit. }
@@ -112,7 +134,7 @@ Proof.
 Qed.
 
 Lemma red_transf_subst1 : forall m1 m2 b v t w,
-  red m1 (transf_rm_pz (subst1 b v t)) m2 w -> 
+  red m1 (transf_rm_pz (subst1 b v t)) m2 w ->
   red m1 (subst1 b v (transf_rm_pz t)) m2 w.
 Proof.
 Admitted.
@@ -127,7 +149,7 @@ Proof.
     { eauto. }
     { case_if*. } }
   { applys* red_let. applys* red_transf_subst1.  }
-  { } 
+  { }
 
 (*
   intros t s1 s2 v. generalize s1, s2, v.
@@ -136,13 +158,13 @@ Proof.
   - simpl. trivial.
   - simpl. trivial.
   (* Fix *)
-  - admit. 
+  - admit.
   (* If *)
   - admit.
-  (* Let *) 
-  - simpl. inversion 1. applys red_let. 
+  (* Let *)
+  - simpl. inversion 1. applys red_let.
     + apply IHt1 in H6. exact H6.
-    + apply subst_inert_in_red in H7. apply IHt2 in H7. 
+    + apply subst_inert_in_red in H7. apply IHt2 in H7.
       apply subst_inert_in_red. exact H7.
 Admitted.*)
 
