Semantics.v
@@ -1,0 +1,357 @@
+(**
+
+This file describes the syntax and semantics of a lambda calculus
+with mutable heap. The language includes recursive functions, and a
+couple of primitive functions. Records and arrays operations are
+encoded using pointer arithmetics, and using the [alloc] operation
+which allocates at once a requested number of consecutive memory cells.
+
+Author: Arthur Charguéraud.
+License: MIT.
+
+*)
+
+Set Implicit Arguments.
+Require Export LibString LibList LibCore.
+Require Export Fmap Bind TLCbuffer.
+Open Scope string_scope.
+
+
+(* ********************************************************************** *)
+(* * Source language syntax *)
+
+
+(* ---------------------------------------------------------------------- *)
+(** Representation of locations and fields *)
+
+Definition loc := nat.
+
+Definition null : loc := 0%nat.
+
+Definition field := var.
+
+Global Opaque field loc.
+
+
+(* ---------------------------------------------------------------------- *)
+(** Grammar of types *)
+
+Definition size := nat.
+
+Inductive typ : Type :=
+  | typ_int : typ
+  | type_double : typ
+  | type_array : size -> typ
+  | typ_var : var -> typ.
+
+Inductive typdef : Type :=
+  | typdef_struct : fmap field typ -> typdef.
+
+Definition typvar := var.
+
+Definition typctx := fmap typvar typdef.
+
+
+(* ---------------------------------------------------------------------- *)
+(** Syntax of the source language *)
+
+Inductive binop : Type :=
+  | binop_eq : binop
+  | binop_sub : binop
+  | binop_add : binop
+  | binop_ptr_add : binop.
+
+Inductive prim : Type :=
+  | prim_binop : binop -> prim
+  | prim_ptr_new : typ -> prim
+  | prim_ptr_get : typ -> prim
+  | prim_ptr_set : typ -> prim
+  | prim_struct_new : typ -> list field -> prim
+  | prim_struct_get : typ -> field -> prim
+  | prim_struct_set : typ -> field -> prim
+  | prim_array_new : typ -> prim
+  | prim_array_get : typ -> prim
+  | prim_array_set : typ -> prim.
+
+Inductive val : Type :=
+  | val_unit : val
+  | val_bool : bool -> val
+  | val_int : int -> val
+  | val_loc : loc -> val
+  | val_prim : prim -> val.
+
+Inductive trm : Type :=
+  | trm_var : var -> trm
+  | trm_val : val -> trm
+  | trm_if : trm -> trm -> trm -> trm
+  | trm_let : bind -> trm -> trm -> trm
+  | trm_app : prim -> list trm -> trm.
+  (*
+  | trm_while : trm -> trm -> trm
+  | trm_for : var -> trm -> trm -> trm -> trm
+  *)
+
+
+(** Sequence is a special case of let bindings *)
+
+Notation trm_seq := (trm_let bind_anon).
+
+(** The type of values is inhabited *)
+
+Global Instance Inhab_val : Inhab val.
+Proof using. apply (Inhab_of_val val_unit). Qed.
+
+(** Shorthand [vars], [vals] and [trms] for lists of items. *)
+
+Definition vals : Type := list val.
+Definition trms : Type := list trm.
+
+
+(* ---------------------------------------------------------------------- *)
+(** Coercions *)
+
+Coercion prim_binop : binop >-> prim.
+Coercion val_prim : prim >-> val.
+Coercion val_bool : bool >-> val.
+Coercion val_int : Z >-> val.
+Coercion val_loc : loc >-> val.
+Coercion trm_val : val >-> trm.
+Coercion trm_var : var >-> trm.
+Coercion trm_app : prim >-> Funclass.
+
+Coercion trms_vals (vs:vals) : trms :=
+  List.map trm_val vs.
+
+
+(* ---------------------------------------------------------------------- *)
+(** Induction principle *)
+
+
+(** An induction principle for trees *)
+
+Section Trm_induct.
+
+Variables
+(P : trm -> Prop)
+(Q : trms -> Prop)
+(P1: forall v : var, P v)
+(P2: forall v : val, P v)
+(P3: forall t : trm, P t -> forall t0 : trm, P t0 -> forall t1 : trm, P t1 -> P (trm_if t t0 t1))
+(P4: forall (b : bind) (t : trm), P t -> forall t0 : trm, P t0 -> P (trm_let b t t0))
+(P5: forall (f : prim) (l : list trm), Q l -> P (trm_app f l))
+(Q1: Q nil)
+(Q2: forall t l, P t -> Q l -> Q (t::l)).
+
+Fixpoint trm_induct_gen (t : trm) : P t :=
+  let F := trm_induct_gen in
+  match t as x return P x with
+  | trm_var v => P1 v
+  | trm_val v => P2 v
+  | trm_if t0 t1 t2 => P3 (F t0) (F t1) (F t2)
+  | trm_let b t0 t1 => P4 b (F t0) (F t1)
+  | trm_app f l => P5 f 
+      ((fix trms_induct (l : trms) : Q l :=
+      match l as x return Q x with
+      | nil   => Q1
+      | t::l' => Q2 (F t) (trms_induct l')
+      end) l)
+  end.
+
+End Trm_induct.
+
+(* To use it:
+  eapply tree_induct_gen with (Q := fun l =>
+    forall t, Mem t l -> P t);
+*)
+
+
+(* ********************************************************************** *)
+(* * Low-level semantics *)
+
+(* LATER
+
+Definition typsize := nat.
+
+Definition typctxsize := fmap typvar typsize.
+
+Definition sizeof (C:typctx) (T:typ) : typsize :=
+  match T with
+  | typ_int => 1%nat
+  | typ_double => 2%nat
+  | typ_var X =>
+    match fmap_data C X with
+    | Some n => n
+    | None => 0%nat (* or [arbitrary] *)
+    end
+  end.
+
+*)
+
+
+
+(* ********************************************************************** *)
+(* * Source language semantics *)
+
+(* ---------------------------------------------------------------------- *)
+(** Big-step evaluation *)
+
+Implicit Types t : trm.
+Implicit Types v : val.
+Implicit Types l : loc.
+Implicit Types i : field.
+Implicit Types b : bool.
+Implicit Types n : int.
+Implicit Types x : var.
+Implicit Types z : bind.
+Implicit Types vs : vals.
+Implicit Types ts : trms.
+
+Definition state := fmap loc val.
+
+Definition env := Ctx.ctx val.
+
+Section Red.
+
+Definition is_val t :=
+  match t with
+  | trm_val v => True
+  | _ => False
+  end.
+
+Local Open Scope fmap_scope.
+
+Inductive redbinop : binop -> val -> val -> val -> Prop :=
+  | redbinop_add : forall n1 n2,
+      redbinop binop_add (val_int n1) (val_int n2) (val_int (n1 + n2))
+  | redbinop_sub : forall n1 n2,
+      redbinop binop_sub (val_int n1) (val_int n2) (val_int (n1 - n2))
+  | redbinop_ptr_add : forall l' l n,
+      (l':nat) = (l:nat) + n :> int ->
+      redbinop binop_ptr_add (val_loc l) (val_int n) (val_loc l')
+  | redbinop_eq : forall v1 v2,
+      redbinop binop_eq v1 v2 (val_bool (isTrue (v1 = v2))).
+
+
+Inductive red : env -> state -> trm -> state -> val -> Prop :=
+  | red_var : forall E m v x,
+      Ctx.lookup x E = Some v ->
+      red E m (trm_var x) m v
+  | red_val : forall E m v,
+      red E m v m v
+  | red_if : forall E m1 m2 m3 b r t0 t1 t2,
+      red E m1 t0 m2 (val_bool b) ->
+      red E m2 (if b then t1 else t2) m3 r ->
+      red E m1 (trm_if t0 t1 t2) m3 r
+  | red_let : forall E m1 m2 m3 z t1 t2 v1 r,
+      red E m1 t1 m2 v1 ->
+      red (Ctx.add z v1 E) m2 t2 m3 r ->
+      red E m1 (trm_let z t1 t2) m3 r
+  (* Binary operations *)
+  | red_binop : forall E (op:binop) m v1 v2 v,
+      redbinop op v1 v2 v ->
+      red E m (trm_app op ((trm_val v1)::(trm_val v2)::nil)) m v
+  (* Operations on the heap *)
+  | red_ptr_new : forall E ma mb v l T,
+      mb = (fmap_single l v) ->
+      l <> null ->
+      \# ma mb ->
+      red E ma (trm_app (prim_ptr_new T) (trm_val v::nil)) (mb \+ ma) (val_loc l)
+  | red_ptr_get : forall E m l v T,
+      fmap_data m l = Some v ->
+      red E m (trm_app (prim_ptr_get T) ((trm_val l)::nil)) m v
+  | red_ptr_set : forall E m m' l v T,
+      m' = fmap_update m l v ->
+      red E m (trm_app (prim_ptr_set T) ((trm_val l)::(trm_val v)::nil)) m' val_unit.
+
+  (* | red_arg : forall E m1 m2 m3 f vs ts t1 v1 r,
+      ~ is_val t1 ->
+      red E m1 t1 m2 v1 ->
+      red E m2 (trm_app f ((trms_vals vs)++(trm_val v1)::ts)) m3 r ->
+      red E m1 (trm_app f ((trms_vals vs)++t1::ts)) m3 r *)
+  (* Generic function calls -- later
+      | red_call : forall E m1 m2 m3 m4 t1 t2 f z t3 v1 r,
+      ... execute body of f ...
+      red E m1 (trm_app f vs) m3 r
+   *)
+
+End Red.
+
+
+(* Derived *)
+
+Lemma red_seq : forall E m1 m2 m3 t1 t2 r1 r,
+  red E m1 t1 m2 r1 ->
+  red E m2 t2 m3 r ->
+  red E m1 (trm_seq t1 t2) m3 r.
+Proof using. intros. applys* red_let. Qed.
+
+
+
+(* ********************************************************************** *)
+(* * Notation for terms *)
+
+(* ---------------------------------------------------------------------- *)
+(** Notation for concrete programs *)
+
+Module NotationForTerms.
+
+(** Note: below, many occurences of [x] have type [bind], and not [var] *)
+
+Notation "'()" := val_unit : trm_scope.
+
+Notation "'If_' t0 'Then' t1 'Else' t2" :=
+  (trm_if t0 t1 t2)
+  (at level 69, t0 at level 0) : trm_scope.
+
+Notation "'If_' t0 'Then' t1 'End'" :=
+  (trm_if t0 t1 val_unit)
+  (at level 69, t0 at level 0) : trm_scope.
+
+Notation "'Let' x ':=' t1 'in' t2" :=
+  (trm_let x t1 t2)
+  (at level 69, x at level 0, right associativity,
+  format "'[v' '[' 'Let'  x  ':='  t1  'in' ']'  '/'  '[' t2 ']' ']'") : trm_scope.
+
+Notation "t1 ;;; t2" :=
+  (trm_seq t1 t2)
+  (at level 68, right associativity, only parsing,
+   format "'[v' '[' t1 ']'  ;;;  '/'  '[' t2 ']' ']'") : trm_scope.
+
+(*
+Notation "'ref t" :=
+  (val_ref t)
+  (at level 67) : trm_scope.
+
+Notation "'! t" :=
+  (val_get t)
+  (at level 67) : trm_scope.
+
+Notation "t1 ':= t2" :=
+  (val_set t1 t2)
+  (at level 67) : trm_scope.
+
+Notation "t1 '+ t2" :=
+  (trm_app binop_add (t1::t2::nil))
+  (at level 69) : trm_scope.
+
+Notation "t1 '- t2" :=
+  (trm_binop binop_sub t1 t2)
+  (at level 69) : trm_scope.
+
+Notation "t1 '= t2" :=
+  (trm_binop binop_eq t1 t2)
+  (at level 69) : trm_scope.
+*)
+
+(* Demo for the above notation:
+
+  Open Scope trm_scope.
+  Import NotationForVariables.
+  Definition test := Let 'x := val_unit in val_unit.
+*)
+
+End NotationForTerms.
+
+
+
+
